Mostly ready for h/w synthesis.

examples/dev/AES/aesScript.sml
@@ -8,7 +8,7 @@ struct
 (*
   app load ["RoundOpTheory", "metisLib"];
 *)
-open HolKernel boolLib bossLib RoundOpTheory pairTools metisLib;
+open HolKernel Parse boolLib bossLib RoundOpTheory pairTheory metisLib;
 
 (*---------------------------------------------------------------------------*)
 (* Make bindings to pre-existing stuff                                       *)
@@ -16,108 +16,116 @@ open HolKernel boolLib bossLib RoundOpTheory pairTools metisLib;
 
 val RESTR_EVAL_TAC = computeLib.RESTR_EVAL_TAC;
 
-val BLOCK_VAR_TAC = PGEN_TAC (Term `(b0,b1,b2,b3,b4,b5,b6,b7,b8,
-                                     b9,b10,b11,b12,b13,b14,b15):block`);
-
 val _ = new_theory "aes";
 
 (*---------------------------------------------------------------------------*)
-(* Orchestrate the round computations.                                       *)
-(* Similar to:                                                               *)
-(*                                                                           *)
-(* (Round 0 [key] state = AddRoundKey key (ShiftRows (SubBytes state))) /\   *)
-(* (Round (SUC n) (key::keys) state =                                        *)
-(*     Round n keys                                                          *)
-(*        (AddRoundKey key                                                   *)
-(*             (MixColumns                                                   *)
-(*               (ShiftRows (SubBytes state)))))`;                           *)
+(* The keyschedule can be represented as a circular buffer of fixed size.    *)
+(* It has 11 keys (blocks) in it, and the buffer gets rotated each time      *)
+(* a key is taken from it.                                                   *)
 (*---------------------------------------------------------------------------*)
+
+val _ = 
+  type_abbrev ("keysched",
+    Type `:key#key#key#key#key#key#key#key#key#key#key`);
+
+val FORALL_KEYSCHED = Q.prove
+(`(!x:keysched. P x) = !k1 k2 k3 k4 k5 k6 k7 k8 k9 k10 k11. 
+                        P(k1,k2,k3,k4,k5,k6,k7,k8,k9,k10,k11)`,
+ EQ_TAC THEN RW_TAC std_ss [] THEN
+ `?a1 a2 a3 a4 a5 a6 a7 a8 a9 a10 a11. 
+     x = (a1,a2,a3,a4,a5,a6,a7,a8,a9,a10,a11)`
+   by METIS_TAC [ABS_PAIR_THM]
+ THEN ASM_REWRITE_TAC[]);
+
+
+val ROTKEYS_def = 
+ Define
+   `ROTKEYS (k0,k1,k2,k3,k4,k5,k6,k7,k8,k9,k10) =
+            (k1,k2,k3,k4,k5,k6,k7,k8,k9,k10,k0) : keysched`;
+
+val REVKEYS_def = 
+ Define
+   `REVKEYS (k0,k1,k2,k3,k4,k5,k6,k7,k8,k9,k10) =
+            (k10,k9,k8,k7,k6,k5,k4,k3,k2,k1,k0) : keysched`;
+
+val LIST_TO_KEYS_def = 
+ Define
+  `(LIST_TO_KEYS [] acc = acc) /\
+   (LIST_TO_KEYS (h::t) (k1,k2,k3,k4,k5,k6,k7,k8,k9,k10,k11) =
+         LIST_TO_KEYS t (h,k1,k2,k3,k4,k5,k6,k7,k8,k9,k10))`;
+
+val DUMMY_KEYS_def = 
+ Define
+  `DUMMY_KEYS = (ZERO_BLOCK,ZERO_BLOCK,ZERO_BLOCK,ZERO_BLOCK,
+                 ZERO_BLOCK, ZERO_BLOCK,ZERO_BLOCK,ZERO_BLOCK,
+                 ZERO_BLOCK,ZERO_BLOCK,ZERO_BLOCK)`;
+
+(*---------------------------------------------------------------------------*)
+(* Orchestrate the round computations.                                       *)
+(*---------------------------------------------------------------------------*)
+
 
 val (Round_def, Round_ind) = Defn.tprove
  (Hol_defn 
    "Round"
-   `Round n keys state = 
+   `Round n (keys:keysched) (state:state) = 
      if n=0 
-      then (case keys 
-             of [key] -> AddRoundKey key (ShiftRows (SubBytes state)))
-      else (case keys
-             of k::rst -> Round (n-1) rst
-                             (AddRoundKey k (MixColumns 
-                                 (ShiftRows (SubBytes state)))))`,
+      then AddRoundKey (FST keys) (ShiftRows (SubBytes state))
+      else Round (n-1) (ROTKEYS keys)
+            (AddRoundKey (FST keys) 
+              (MixColumns (ShiftRows (SubBytes state))))`,
   WF_REL_TAC `measure FST`);
 
-val _ = save_thm ("Round_def", Round_def);
-val _ = save_thm ("Round_ind", Round_ind);
-
-(*---------------------------------------------------------------------------*)
-(*  (InvRound 0 [key] state = AddRoundKey key                                *)
-(*                               (InvSubBytes(InvShiftRows state))) /\       *)
-(*  (InvRound n (key::keys) state =                                          *)
-(*      InvRound (n-1) keys                                                  *)
-(*         (InvMixColumns (AddRoundKey key                                   *)
-(*              (InvSubBytes (InvShiftRows state)))))`                       *)
-(*---------------------------------------------------------------------------*)
 
 val (InvRound_def,InvRound_ind) = Defn.tprove
  (Hol_defn 
    "InvRound"
    `InvRound n keys state =
       if n=0 
-       then (case keys 
-              of [key] -> AddRoundKey key 
-                            (InvSubBytes
-                               (InvShiftRows state)))
-       else (case keys
-              of k::rst -> InvRound (n-1) rst
-                              (InvMixColumns 
-                                 (AddRoundKey k 
-                                   (InvSubBytes 
-                                     (InvShiftRows state)))))`,
+       then AddRoundKey (FST keys) (InvSubBytes (InvShiftRows state))
+       else InvRound (n-1) (ROTKEYS keys)
+             (InvMixColumns 
+               (AddRoundKey (FST keys) (InvSubBytes (InvShiftRows state))))`,
   WF_REL_TAC `measure FST`);
 
+val _ = save_thm ("Round_def", Round_def);
+val _ = save_thm ("Round_ind", Round_ind);
 val _ = save_thm ("InvRound_def", InvRound_def);
 val _ = save_thm ("InvRound_ind", InvRound_ind);
 
 (*---------------------------------------------------------------------------*)
-(* The following versions are better for computeLib                          *)
+(* Encrypt and Decrypt                                                       *)
 (*---------------------------------------------------------------------------*)
 
-val Round_eqns = Q.store_thm
- ("Round_eqns",
-  `Round n keys state = 
-     if n=0 
-      then if LENGTH keys = 1 
-             then AddRoundKey (HD keys) (ShiftRows (SubBytes state))
-             else ARB
-      else if NULL keys then ARB
-             else Round (n-1) (TL keys)
-                   (AddRoundKey (HD keys) 
-                     (MixColumns (ShiftRows (SubBytes state))))`,
- Cases_on `keys` 
-   THEN CONV_TAC (LHS_CONV (ONCE_REWRITE_CONV [Round_def]))
-   THEN RW_TAC list_ss [listTheory.LENGTH_NIL]
-   THEN Cases_on `t` THEN FULL_SIMP_TAC list_ss []);
+val AES_FWD_def = 
+ Define 
+  `AES_FWD keys = 
+    from_state o Round 9 (ROTKEYS keys) o AddRoundKey (FST keys) o to_state`;
+     
 
+val AES_BWD_def = 
+ Define 
+  `AES_BWD keys = 
+    from_state o InvRound 9 (ROTKEYS keys) o AddRoundKey (FST keys) o to_state`;
+     
+(*---------------------------------------------------------------------------*)
+(* Main lemma                                                                *)
+(*---------------------------------------------------------------------------*)
 
-val InvRound_eqns = Q.store_thm
- ("InvRound_eqns",
-  `InvRound n keys state =
-      if n=0 
-       then if LENGTH keys = 1
-              then AddRoundKey (HD keys) (InvSubBytes (InvShiftRows state))
-              else ARB
-       else if NULL keys then ARB
-              else InvRound (n-1) (TL keys)
-                    (InvMixColumns 
-                       (AddRoundKey (HD keys) 
-                          (InvSubBytes (InvShiftRows state))))`,
- Cases_on `keys` 
-   THEN CONV_TAC (LHS_CONV (ONCE_REWRITE_CONV [InvRound_def]))
-   THEN RW_TAC list_ss [listTheory.LENGTH_NIL]
-   THEN Cases_on `t` THEN FULL_SIMP_TAC list_ss []);
+val [MultCol] = decls "MultCol";
+val [InvMultCol] = decls "InvMultCol";
+val [genMixColumns] = decls "genMixColumns";
 
-val _ = computeLib.add_persistent_funs [("Round_eqns",Round_eqns)];
-val _ = computeLib.add_persistent_funs [("InvRound_eqns",InvRound_eqns)];
+val AES_LEMMA = Q.store_thm
+("AES_LEMMA",
+ `!(plaintext:state) (keys:keysched). 
+     AES_BWD (REVKEYS keys) (AES_FWD keys plaintext) = plaintext`,
+ SIMP_TAC std_ss [FORALL_BLOCK] THEN 
+ SIMP_TAC std_ss [FORALL_KEYSCHED]
+   THEN RESTR_EVAL_TAC [MultCol,InvMultCol,genMixColumns]
+   THEN RW_TAC std_ss [ShiftRows_Inversion,SubBytes_Inversion,
+                       XOR_BLOCK_IDEM,MixColumns_Inversion,
+                       from_state_Inversion,from_state_def]);
 
 
 (*---------------------------------------------------------------------------
@@ -127,12 +135,9 @@ val _ = computeLib.add_persistent_funs [("InvRound_eqns",InvRound_eqns)];
      order that the state also has.
  ---------------------------------------------------------------------------*)
 
-val XOR8x4_def = Define `(a,b,c,d) XOR8x4 (a1,b1,c1,d1) 
-                                     = 
-                                 (a XOR8 a1, 
-                                  b XOR8 b1, 
-                                  c XOR8 c1, 
-                                  d XOR8 d1)`;
+val XOR8x4_def = 
+ Define 
+   `(a,b,c,d) XOR8x4 (a1,b1,c1,d1) = (a # a1, b # b1, c # c1, d # d1)`;
 
 val SubWord_def = Define 
    `SubWord(b0,b1,b2,b3) = (Sbox b0, Sbox b1, Sbox b2, Sbox b3)`;
@@ -172,10 +177,20 @@ val _ = computeLib.add_persistent_funs [("expand_def", expand_def)];
 
 val mk_keysched_def = Define
  `mk_keysched ((b0,b1,b2,b3,b4,b5,b6,b7,b8,b9,b10,b11,b12,b13,b14,b15):key)
-    = 
+      = 
   expand 4 [(b12,b13,b14,b15) ; (b8,b9,b10,b11) ;
             (b4,b5,b6,b7)     ; (b0,b1,b2,b3)]`;
 
+
+(*---------------------------------------------------------------------------*)
+(* Sanity check                                                              *)
+(*---------------------------------------------------------------------------*)
+
+val keysched_length = Count.apply Q.prove
+(`!key. LENGTH (mk_keysched key) = 11`,
+ SIMP_TAC std_ss [FORALL_BLOCK,mk_keysched_def]
+  THEN REPEAT GEN_TAC 
+  THEN EVAL_TAC);
 
 (*---------------------------------------------------------------------------*)
 (* Generate key schedule, and its inverse, then build the encryption and     *)
@@ -184,436 +199,23 @@ val mk_keysched_def = Define
 (*---------------------------------------------------------------------------*)
 
 val AES_def = Define
- `AES key =
-   let sched = mk_keysched key in
-   let isched = REVERSE sched 
-   in
-     ((from_state o Round 9 (TL sched) 
-                  o AddRoundKey (HD sched) o to_state),
-      (from_state o InvRound 9 (TL isched) 
-                  o AddRoundKey (HD isched) o to_state))`;
-
-
-(*---------------------------------------------------------------------------*)
-(* Now let's show that it works for all inputs                               *)
-(*---------------------------------------------------------------------------*)
-
-
-(*---------------------------------------------------------------------------*)
-(* expand is tail recursive and adds a new element to its accumulator at     *)
-(* each recursive call.                                                      *)
-(*---------------------------------------------------------------------------*)
-
-val lemma = Q.prove
-(`!n t. 
-    3 < n /\ n < 44 
-      ==> 
-    ?h. expand (n+1) (h::t) = expand n t`,
- RW_TAC std_ss []
-   THEN GEN_REWRITE_TAC (BINDER_CONV o RHS_CONV) empty_rewrites [expand_def]
-   THEN RW_TAC arith_ss [LET_THM]
-   THEN METIS_TAC []);
-
-
-(*---------------------------------------------------------------------------*)
-(* Build special purpose proof support for next lemma.                       *)
-(*---------------------------------------------------------------------------*)
-
-fun inst_lemma_tac i (asl,w) =
-  let open numSyntax boolSyntax
-      val j = term_of_int i
-      val num_eq = DECIDE (Term `^j + 1 = ^(term_of_int (i+1))`)
-      val ineq   = DECIDE (Term `3 < ^j /\ ^j < 44`)
-      val lem = GSYM (simpLib.SIMP_RULE std_ss [num_eq,ineq] (SPEC j lemma))
-      val pat = lhs(snd(dest_exists(snd(strip_forall (concl lem)))))
-      val theta = match_term pat (find_term (can (match_term pat)) w)
-  in
-    CHOOSE_THEN (fn th => PURE_REWRITE_TAC [th]) 
-                (INST (fst theta) (SPEC_ALL lem)) (asl,w)
-  end;
-
-val expand_4_lemma = Lib.with_flag(Globals.priming,SOME "")
-Q.prove
- (`!a b c d.
-   ?h1 h2 h3 h4 h5 h6 h7 h8 h9 h10
-    h11 h12 h13 h14 h15 h16 h17 h18 h19 h20 
-    h21 h22 h23 h24 h25 h26 h27 h28 h29 h30
-    h31 h32 h33 h34 h35 h36 h37 h38 h39 h40. 
-     expand 44 [h40;h39;h38;h37;h36;h35;h34;h33;h32;h31;h30;h29;h28;
-                h27;h26;h25;h24;h23;h22;h21;h20;h19;h18;h17;h16;h15;
-                h14;h13;h12;h11;h10;h9;h8;h7;h6;h5;h4;h3;h2;h1;a;b;c;d]
-        = 
-     expand 4 [a;b;c;d]`,
-  REPEAT GEN_TAC 
-    THEN EVERY (map inst_lemma_tac (upto 4 43)) 
-    THEN PROVE_TAC []);
-
-(*---------------------------------------------------------------------------*)
-(* Surprisingly complicated to calculate the length of the list produced by  *)
-(* mk_keysched.                                                              *)
-(*---------------------------------------------------------------------------*)
-
-val keysched_length = Q.prove
-(`!key. LENGTH (mk_keysched key) = 11`,
- PGEN_TAC (Term `(b0,b1,b2,b3,b4,b5,b6,b7,b8,b9,b10,b11,b12,b13,b14,b15):key`) 
-  THEN REWRITE_TAC [mk_keysched_def]
-  THEN STRIP_ASSUME_TAC 
-       (GSYM (Q.SPECL [`(b12,b13,b14,b15)`, `(b8,b9,b10,b11)`, 
-                       `(b4,b5,b6,b7)`,     `(b0,b1,b2,b3)`] expand_4_lemma))
-  THEN ASM_REWRITE_TAC[]
-  THEN POP_ASSUM (K ALL_TAC)
-  THEN EVAL_TAC
-  THEN MAP_EVERY Q.ID_SPEC_TAC  
-   [`h1`,  `h2`,  `h3`,  `h4`,  `h5`,  `h6`,  `h7`,  `h8`,  `h9`,  `h10`,
-    `h11`, `h12`, `h13`, `h14`, `h15`, `h16`, `h17`, `h18`, `h19`, `h20`, 
-    `h21`, `h22`, `h23`, `h24`, `h25`, `h26`, `h27`, `h28`, `h29`, `h30`,
-    `h31`, `h32`, `h33`, `h34`, `h35`, `h36`, `h37`, `h38`, `h39`, `h40`]
-  THEN PGEN_TAC (Term`(h1a,h1b,h1c,h1d):w8x4`)
-  THEN PGEN_TAC (Term`(h2a,h2b,h2c,h2d):w8x4`)
-  THEN PGEN_TAC (Term`(h3a,h3b,h3c,h3d):w8x4`)
-  THEN PGEN_TAC (Term`(h4a,h4b,h4c,h4d):w8x4`)
-  THEN PGEN_TAC (Term`(h5a,h5b,h5c,h5d):w8x4`)
-  THEN PGEN_TAC (Term`(h6a,h6b,h6c,h6d):w8x4`)
-  THEN PGEN_TAC (Term`(h7a,h7b,h7c,h7d):w8x4`)
-  THEN PGEN_TAC (Term`(h8a,h8b,h8c,h8d):w8x4`)
-  THEN PGEN_TAC (Term`(h9a,h9b,h9c,h9d):w8x4`)
-  THEN PGEN_TAC (Term`(h10a,h10b,h10c,h10d):w8x4`)
-  THEN PGEN_TAC (Term`(h11a,h11b,h11c,h11d):w8x4`)
-  THEN PGEN_TAC (Term`(h12a,h12b,h12c,h12d):w8x4`)
-  THEN PGEN_TAC (Term`(h13a,h13b,h13c,h13d):w8x4`)
-  THEN PGEN_TAC (Term`(h14a,h14b,h14c,h14d):w8x4`)
-  THEN PGEN_TAC (Term`(h15a,h15b,h15c,h15d):w8x4`)
-  THEN PGEN_TAC (Term`(h16a,h16b,h16c,h16d):w8x4`)
-  THEN PGEN_TAC (Term`(h17a,h17b,h17c,h17d):w8x4`)
-  THEN PGEN_TAC (Term`(h18a,h18b,h18c,h18d):w8x4`)
-  THEN PGEN_TAC (Term`(h19a,h19b,h19c,h19d):w8x4`)
-  THEN PGEN_TAC (Term`(h20a,h20b,h20c,h20d):w8x4`)
-  THEN PGEN_TAC (Term`(h21a,h21b,h21c,h21d):w8x4`)
-  THEN PGEN_TAC (Term`(h22a,h22b,h22c,h22d):w8x4`)
-  THEN PGEN_TAC (Term`(h23a,h23b,h23c,h23d):w8x4`)
-  THEN PGEN_TAC (Term`(h24a,h24b,h24c,h24d):w8x4`)
-  THEN PGEN_TAC (Term`(h25a,h25b,h25c,h25d):w8x4`)
-  THEN PGEN_TAC (Term`(h26a,h26b,h26c,h26d):w8x4`)
-  THEN PGEN_TAC (Term`(h27a,h27b,h27c,h27d):w8x4`)
-  THEN PGEN_TAC (Term`(h28a,h28b,h28c,h28d):w8x4`)
-  THEN PGEN_TAC (Term`(h29a,h29b,h29c,h29d):w8x4`)
-  THEN PGEN_TAC (Term`(h30a,h30b,h30c,h30d):w8x4`)
-  THEN PGEN_TAC (Term`(h31a,h31b,h31c,h31d):w8x4`)
-  THEN PGEN_TAC (Term`(h32a,h32b,h32c,h32d):w8x4`)
-  THEN PGEN_TAC (Term`(h33a,h33b,h33c,h33d):w8x4`)
-  THEN PGEN_TAC (Term`(h34a,h34b,h34c,h34d):w8x4`)
-  THEN PGEN_TAC (Term`(h35a,h35b,h35c,h35d):w8x4`)
-  THEN PGEN_TAC (Term`(h36a,h36b,h36c,h36d):w8x4`)
-  THEN PGEN_TAC (Term`(h37a,h37b,h37c,h37d):w8x4`)
-  THEN PGEN_TAC (Term`(h38a,h38b,h38c,h38d):w8x4`)
-  THEN PGEN_TAC (Term`(h39a,h39b,h39c,h39d):w8x4`)
-  THEN PGEN_TAC (Term`(h40a,h40b,h40c,h40d):w8x4`)
-  THEN EVAL_TAC);
-
-val length_11 = 
- Lib.with_flag(Globals.priming,SOME "")
-  Q.prove
- (`!l. (LENGTH l = 11) = 
-       ?h1 h2 h3 h4 h5 h6 h7 h8 h9 h10 h11.
-         l = [h1;h2;h3;h4;h5;h6;h7;h8;h9;h10;h11]`,
- GEN_TAC THEN EQ_TAC THENL
- [Cases_on `l`  THEN EVAL_TAC THEN
-  Cases_on `t`  THEN EVAL_TAC THEN
-  Cases_on `t1` THEN EVAL_TAC THEN
-  Cases_on `t`  THEN EVAL_TAC THEN
-  Cases_on `t1` THEN EVAL_TAC THEN
-  Cases_on `t`  THEN EVAL_TAC THEN
-  Cases_on `t1` THEN EVAL_TAC THEN
-  Cases_on `t`  THEN EVAL_TAC THEN
-  Cases_on `t1` THEN EVAL_TAC THEN
-  Cases_on `t`  THEN EVAL_TAC THEN
-  Cases_on `t1` THEN EVAL_TAC THEN
-  Cases_on `t`  THEN EVAL_TAC THENL [PROVE_TAC [], DECIDE_TAC],
- RW_TAC list_ss [] THEN EVAL_TAC]);
-
-
-(*---------------------------------------------------------------------------*)
-(* Main lemma                                                                *)
-(*---------------------------------------------------------------------------*)
-
-val [MultCol] = decls "MultCol";
-val [InvMultCol] = decls "InvMultCol";
-val [genMixColumns] = decls "genMixColumns";
-
-val lemma = Q.prove
-(`!plaintext : state. 
-  !sched rsched:state list. 
-    (LENGTH sched = 11) /\ (rsched = REVERSE sched)
-        ==>
-    ((from_state
-       o InvRound 9 (TL rsched) 
-       o AddRoundKey (HD rsched) 
-       o to_state
-       o from_state
-       o Round 9 (TL sched) 
-       o AddRoundKey (HD sched) 
-       o to_state) plaintext = plaintext)`,
- BLOCK_VAR_TAC THEN RW_TAC std_ss [length_11]
-   THEN RESTR_EVAL_TAC [MultCol,InvMultCol,genMixColumns]
-   THEN RW_TAC std_ss [ShiftRows_Inversion,SubBytes_Inversion,
-                       XOR_BLOCK_IDEM,MixColumns_Inversion,
-                       from_state_Inversion,from_state_def]);
+ `AES key = 
+   let keys = LIST_TO_KEYS (mk_keysched key) DUMMY_KEYS 
+   in (AES_FWD keys, AES_BWD (REVKEYS keys))`;
 
 
 (*---------------------------------------------------------------------------*)
 (* Basic theorem about encryption/decryption                                 *)
 (*---------------------------------------------------------------------------*)
 
-val AES_Correct = Q.store_thm
-  ("AES_Correct",
+val AES_CORRECT = Q.store_thm
+  ("AES_CORRECT",
    `!key plaintext. 
        ((encrypt,decrypt) = AES key)
        ==>
        (decrypt (encrypt plaintext) = plaintext)`,
-   RW_TAC std_ss [AES_def,GSYM combinTheory.o_ASSOC, LET_THM] THEN
-   RW_TAC std_ss [combinTheory.o_THM] THEN
-   PROVE_TAC [SIMP_RULE std_ss [combinTheory.o_THM] lemma, keysched_length]);
+ RW_TAC std_ss [AES_def,LET_THM,AES_LEMMA]);
 
-
-(*===========================================================================*)
-(* Alternative decryption approach and its correctness                       *)
-(*===========================================================================*)
-
-
-(*---------------------------------------------------------------------------*)
-(* Map InvMixColumns over the keyschedule before embarking on the            *)
-(* alternative inverse round computation. However, do not alter the first or *)
-(* last element of the keyschedule.                                          *)
-(*---------------------------------------------------------------------------*)
-
-val InvMix_def = Define 
-   `(InvMix [x] = [x]) /\
-    (InvMix (h::t) = InvMixColumns h::InvMix t)`;
-
-val InvMixify_def = Define 
-   `InvMixify (h::t) = h::InvMix t`;
-
-
-(*---------------------------------------------------------------------------*)
-(* Alternative inverse rounds                                                *)
-(*                                                                           *)
-(*  EqInvRound 0 [key] state = AddRoundKey key                               *)
-(*                               (InvShiftRows                               *)
-(*                                 (InvSubBytes state)))                     *)
-(*  EqInvRound n (key::keys) state =                                         *)
-(*      EqInvRound (n-1) keys                                                *)
-(*         (AddRoundKey key                                                  *)
-(*           (InvMixColumns                                                  *)
-(*             (InvShiftRows                                                 *)
-(*               (InvSubBytes state))))                                      *)
-(*---------------------------------------------------------------------------*)
-
-val (EqInvRound_def,EqInvRound_ind) = Defn.tprove
- (Hol_defn 
-   "EqInvRound"
-   `EqInvRound n keys state =
-      if n=0 
-       then (case keys 
-              of [key] -> AddRoundKey key 
-                            (InvShiftRows 
-                               (InvSubBytes(state))))
-       else (case keys
-              of k::rst -> EqInvRound (n-1) rst
-                              (AddRoundKey k 
-                                (InvMixColumns 
-                                  (InvShiftRows
-                                     (InvSubBytes state)))))`,
-  WF_REL_TAC `measure FST`);
-
-val _ = save_thm ("EqInvRound_def",EqInvRound_def);
-val _ = save_thm ("EqInvRound_ind",EqInvRound_ind);
-
-val EqInvRound_eqns = Q.store_thm
-("EqInvRound_eqns",
- `EqInvRound n keys state =
-      if n=0 
-       then if LENGTH keys = 1
-               then AddRoundKey (HD keys) (InvShiftRows (InvSubBytes state))
-               else ARB
-       else if NULL keys then ARB
-              else EqInvRound (n-1) (TL keys)
-                     (AddRoundKey (HD keys)
-                       (InvMixColumns (InvShiftRows (InvSubBytes state))))`,
- Cases_on `keys` 
-   THEN CONV_TAC (LHS_CONV (ONCE_REWRITE_CONV [EqInvRound_def]))
-   THEN RW_TAC list_ss [listTheory.LENGTH_NIL]
-   THEN Cases_on `t` THEN FULL_SIMP_TAC list_ss []);
-
-val _ = computeLib.add_persistent_funs [("EqInvRound_eqns",EqInvRound_eqns)];
-
-(*---------------------------------------------------------------------------*)
-(* Grab some constants (to help control symbolic evaluation)                 *)
-(*---------------------------------------------------------------------------*)
-
-val [InvMixColumns] = decls "InvMixColumns";
-val [InvShiftRows]  = decls "InvShiftRows";
-val [InvSubBytes]   = decls "InvSubBytes";
-val [AddRoundKey]   = decls "AddRoundKey";
-
-(*---------------------------------------------------------------------------*)
-(* Prove the equivalence of the alternative scheme                           *)
-(*---------------------------------------------------------------------------*)
-
-val Equiv_lemma = Q.prove
-(`!sched sched' : state list.
-      (LENGTH sched = 11) /\ (sched' = InvMixify sched)
-      ==> 
-       (EqInvRound 9 (TL sched') o AddRoundKey (HD sched')
-         =
-        InvRound 9 (TL sched) o AddRoundKey (HD sched))`,
-  RW_TAC std_ss [] THEN CONV_TAC FUN_EQ_CONV THEN GEN_TAC 
-    THEN POP_ASSUM MP_TAC 
-    THEN RW_TAC std_ss [length_11]
-    THEN RW_TAC list_ss [InvMixify_def]
-    THEN MATCH_MP_TAC (PROVE [combinTheory.o_THM] 
-           (Term `(!s:state. f s = g s) ==> (f (h s) = g (h s))`))
-    THEN RESTR_EVAL_TAC [InvMixColumns,InvShiftRows,AddRoundKey,InvSubBytes]
-    THEN RW_TAC std_ss [InvShiftRows_InvSubBytes_Commute,
-                        GSYM InvMixColumns_Distrib]);
-
-val LENGTH_REVERSE = Q.prove
-(`!l. LENGTH(REVERSE l) = LENGTH l`,
- Induct THEN RW_TAC list_ss []);
-
-(*---------------------------------------------------------------------------*)
-(* Encrypt as in AES, but use alternative decryptor.                         *)
-(*---------------------------------------------------------------------------*)
-
-val altAES_def = Define
- `altAES key =
-   let sched = mk_keysched key in
-   let isched = InvMixify (REVERSE sched)
-   in
-     ((from_state o Round 9 (TL sched) 
-                  o AddRoundKey (HD sched) o to_state),
-      (from_state o EqInvRound 9 (TL isched) 
-                  o AddRoundKey (HD isched) o to_state))`;
-
-(*---------------------------------------------------------------------------*)
-(* Equality of AES and altAES                                                *)
-(*---------------------------------------------------------------------------*)
-
-val altAES_eq_AES = Q.prove
-(`!k. altAES k = AES k`,
- RW_TAC std_ss [altAES_def, AES_def, LET_THM] THEN
- MATCH_MP_TAC (PROVE [combinTheory.o_THM] 
-                     (Term `(f=g) ==> (h o f = h o g)`)) THEN
- REWRITE_TAC [combinTheory.o_ASSOC] THEN 
- MATCH_MP_TAC (PROVE [combinTheory.o_THM] (Term `(f=g) ==> (f o h = g o h)`))
- THEN RW_TAC std_ss [Equiv_lemma,LENGTH_REVERSE,keysched_length]);
-
-(*---------------------------------------------------------------------------*)
-(* Hence correctness of alternative decryptor                                *)
-(*---------------------------------------------------------------------------*)
-
-val altAES_Correct = Q.store_thm
- ("altAES_Correct",
-  `!key plaintext. 
-       ((encrypt,decrypt) = altAES key)
-        ==>
-        (decrypt (encrypt plaintext) = plaintext)`,
-   PROVE_TAC [AES_Correct,altAES_eq_AES]);
-
-
-
-val Round_def' = Q.prove
-(`Round n keys state = 
-     if n=0 
-      then (case keys 
-             of [key] -> AddRoundKey key (ShiftRows (SubBytes state))
-             || other -> FAIL Round ^(mk_var("need exactly one key",bool))
-                              n keys state)
-      else (case keys
-             of [] -> FAIL Round ^(mk_var("no keys left",bool)) n keys state
-             || k::rst -> Round (n-1) rst
-                             (AddRoundKey k (MixColumns 
-                                 (ShiftRows (SubBytes state)))))`,
- REPEAT CASE_TAC THENL
-   [RW_TAC std_ss [combinTheory.FAIL_THM],
-    RW_TAC std_ss [combinTheory.FAIL_THM],
-    RW_TAC std_ss [Once Round_def],
-    RW_TAC std_ss [Once Round_def],
-    RW_TAC std_ss [combinTheory.FAIL_THM],
-    RW_TAC std_ss [Once Round_def]]);
-
-
-val InvRound_def' = Q.prove
-(`InvRound n keys state =
-      if n=0 
-       then (case keys 
-              of [key] -> AddRoundKey key 
-                            (InvSubBytes
-                               (InvShiftRows state))
-              || other -> FAIL InvRound ^(mk_var("need exactly one key",bool))
-                              n keys state)
-       else (case keys
-              of [] -> FAIL InvRound ^(mk_var("no keys left",bool)) n keys state
-              || k::rst -> InvRound (n-1) rst
-                              (InvMixColumns 
-                                 (AddRoundKey k 
-                                   (InvSubBytes 
-                                     (InvShiftRows state)))))`,
- REPEAT CASE_TAC THENL
-   [RW_TAC std_ss [combinTheory.FAIL_THM],
-    RW_TAC std_ss [combinTheory.FAIL_THM],
-    RW_TAC std_ss [Once InvRound_def],
-    RW_TAC std_ss [Once InvRound_def],
-    RW_TAC std_ss [combinTheory.FAIL_THM],
-    RW_TAC std_ss [Once InvRound_def]]);
-
-
-val EqInvRound_def' = Q.prove
-(`EqInvRound n keys state =
-      if n=0 
-       then (case keys 
-              of [key] -> AddRoundKey key 
-                            (InvShiftRows 
-                               (InvSubBytes(state)))
-              || other -> FAIL EqInvRound ^(mk_var("need exactly one key",bool))
-                              n keys state)
-       else (case keys
-              of [] -> FAIL EqInvRound ^(mk_var("no keys left",bool)) n keys state
-              || k::rst -> EqInvRound (n-1) rst
-                              (AddRoundKey k 
-                                (InvMixColumns 
-                                  (InvShiftRows
-                                     (InvSubBytes state)))))`,
- REPEAT CASE_TAC THENL
-   [RW_TAC std_ss [combinTheory.FAIL_THM],
-    RW_TAC std_ss [combinTheory.FAIL_THM],
-    RW_TAC std_ss [Once EqInvRound_def],
-    RW_TAC std_ss [Once EqInvRound_def],
-    RW_TAC std_ss [combinTheory.FAIL_THM],
-    RW_TAC std_ss [Once EqInvRound_def]]);
-
-val _ = 
-  let open sboxTheory RoundOpTheory EmitML
-  in exportML("aes",
-      MLSTRUCT "type num = numML.num" ::
-      MLSIG "type num = numML.num"
-      :: 
-      map DEFN 
-      [ Sbox_def, InvSbox_def, ZERO_def, ONE_def,TWO_def,THREE_def,
-        NINE_def, ONE_B_def, EIGHTY_def, B_HEX_def, D_HEX_def, E_HEX_def,
-        B2N_def, BYTE_TO_NUM_def, NUM_TO_BYTE_def, 
-        LeftShift_def, RightShift_def, XOR_def, XOR8_def, AND8_def,
-        XOR_BLOCK_def, 
-        to_state_def, from_state_def, 
-        genSubBytes_def, SubBytes_def, InvSubBytes_def,
-        ShiftRows_def, InvShiftRows_def, 
-        xtime_def, ConstMult_def, PolyExp_def, 
-        MultCol_def, InvMultCol_def,
-        genMixColumns_def, MixColumns_def, InvMixColumns_def,
-        AddRoundKey_def, Round_def', InvRound_def', 
-        XOR8x4_def, SubWord_def, RotWord_def, Rcon_def, unpack_def,
-        expand_def, mk_keysched_def, AES_def, 
-        InvMix_def, InvMixify_def, EqInvRound_def', altAES_def])
-  end
 
 val _ = export_theory();
 
